theories/Reductions/FMsetC_to_FMsetEC.v
@@ -22,77 +22,6 @@ From Undecidability Require Import Problems.FMsetC Problems.Reduction.
 From Undecidability Require Import FMset.mset_utils FMset.mset_eq_utils FMset.mset_term_utils.
 Import NatNat.
 
-Lemma nat_to_nat2_non_increasing {n} : fst (nat_to_nat2 n) + snd (nat_to_nat2 n) < S n.
-Proof.
-  elim: n=> [|n] //=.
-  move: (nat_to_nat2 n) => [x y].
-  case: y => [|y]; case: x => [|x] /=; by lia.
-Qed.
-
-Inductive tree : Set :=
-  | leaf : tree
-  | node : nat -> tree -> tree -> tree.
-
-Fixpoint tree_to_nat (t: tree) : nat :=
-  match t with
-  | leaf => 0
-  | node n t u => S (nat2_to_nat (n, nat2_to_nat ((tree_to_nat t), (tree_to_nat u))))
-  end.
-
-Lemma aux1 {n} : (fst (nat_to_nat2 (snd (nat_to_nat2 n)))) < S n.
-Proof. 
-  have ? := @nat_to_nat2_non_increasing n.
-  have ? := @nat_to_nat2_non_increasing (snd (nat_to_nat2 n)).
-  by lia.
-Qed.
-
-Lemma aux2 {n} : (snd (nat_to_nat2 (snd (nat_to_nat2 n)))) < S n.
-Proof. 
-  have ? := @nat_to_nat2_non_increasing n.
-  have ? := @nat_to_nat2_non_increasing (snd (nat_to_nat2 n)).
-  by lia.
-Qed.
-  
-Definition nat_to_tree : nat -> tree.
-Proof.
-  apply: (Fix lt_wf _). case.
-    exact (fun _ => leaf).
-  move=> n f.
-  pose m := snd (nat_to_nat2 n).
-  refine (node (fst (nat_to_nat2 n)) (f (fst (nat_to_nat2 m)) _) (f (snd (nat_to_nat2 m)) _)).
-    exact aux1.
-  exact aux2.
-Defined.
-
-Lemma nat_to_tree_S_nP {n} : 
-  nat_to_tree (S n) = 
-    node (fst (nat_to_nat2 n)) 
-      (nat_to_tree (fst (nat_to_nat2 (snd (nat_to_nat2 n)))))
-      (nat_to_tree (snd (nat_to_nat2 (snd (nat_to_nat2 n))))).
-Proof.
-  rewrite /nat_to_tree Fix_eq=> //. elim=> // *. by f_equal.
-Qed.
-    
-Lemma nat_tree_cancel {t} : nat_to_tree (tree_to_nat t) = t.
-Proof.
-  elim: t=> // *.
-  rewrite /tree_to_nat nat_to_tree_S_nP nat_nat2_cancel.
-  rewrite -/tree_to_nat /fst /snd -/(fst _) -/(snd _) nat_nat2_cancel. 
-  by f_equal.
-Qed.
-    
-Lemma tree_nat_cancel {n} : tree_to_nat (nat_to_tree n) = n.
-Proof.
-  elim /lt_wf_ind: n. case=> //.
-  move=> n IH. rewrite nat_to_tree_S_nP /tree_to_nat -/tree_to_nat ? IH.
-    1,2: have ? := @nat_to_nat2_non_increasing n.
-    1,2: have ? := @nat_to_nat2_non_increasing (snd (nat_to_nat2 n)).
-    1,2: by lia.
-  rewrite - surjective_pairing nat2_nat_cancel.
-  by rewrite - surjective_pairing nat2_nat_cancel.
-Qed.
-
-
 Fixpoint term_to_tree (t: mset_term) : tree :=
   match t with
   | mset_term_zero => node 0 leaf leaf
@@ -137,7 +66,6 @@ Fixpoint term_to_msetcs (t: mset_term) : list msetc :=
       [msetc_h (term_to_nat t) (term_to_nat u)] ++ (term_to_msetcs u)
   end.
 
-
 Definition encode_eq (t u: mset_term) :=
   [(msetc_sum (tree_to_nat leaf) (tree_to_nat leaf) (tree_to_nat leaf)); 
   (msetc_sum (term_to_nat t) (tree_to_nat leaf) (term_to_nat u))].
@@ -145,39 +73,6 @@ Definition encode_eq (t u: mset_term) :=
 (* encode FMsetC_PROBLEM as LPolyNC_PROBLEM *)
 Definition encode_problem (msetcs : FMsetC_PROBLEM) : FMsetEC_PROBLEM :=
   flat_map (fun '(t, u) => (encode_eq t u) ++ term_to_msetcs t ++ term_to_msetcs u) msetcs.
-
-(*
-Section ForallNorm.
-
-Variable T : Type.
-Variable P : T -> Prop.
-
-Lemma Forall_nilP : Forall P [] <-> True.
-Proof. by constructor. Qed.
-
-Lemma Forall_consP {a A} : Forall P (a :: A) <-> P a /\ Forall P A.
-Proof.
-  constructor. 
-    move=> H. by inversion H.
-  move=> [? ?]. by constructor.
-Qed.
-
-Lemma Forall_singletonP {a} : Forall P [a] <-> P a.
-Proof. rewrite Forall_consP Forall_nilP. by tauto. Qed.
-
-Lemma Forall_appP {A B}: Forall P (A ++ B) <-> Forall P A /\ Forall P B.
-Proof.
-  elim: A.
-    constructor; by [|case].
-  move=> ? ? IH /=. rewrite ? Forall_consP ? IH.
-  by tauto.
-Qed.
-
-(* usage rewrite ? Forall_norm *)
-Definition Forall_norm := (@Forall_appP, @Forall_singletonP, @Forall_consP, @Forall_nilP).
-
-End ForallNorm.
-*)
 
 Lemma Forall_flat_mapP {X Y: Type} {P: Y -> Prop} {f: X -> list Y} {A: list X}: 
   Forall P (flat_map f A) <-> Forall (fun a => Forall P (f a)) A.
@@ -226,22 +121,6 @@ Proof.
   by rewrite - ? term_to_nat_pos ? nat_term_cancel.
 Qed.
 
-Print Assumptions completeness.
-
-
-Lemma eq_app_nil_nilP {A} : A ≡ A ++ A -> A = [].
-Proof. Admitted.
-
-Lemma eq_mapI {A B} : A ≡ B -> map S A ≡ map S B.
-Proof.
-  rewrite /mset_eq => + c. move=> /(_ (Nat.pred c)).
-  case: c.
-    admit.
-  move=> c. rewrite - ? (count_occ_map S Nat.eq_dec Nat.eq_dec); first last.
-    done.
-  all: move=> >; by case.
-Admitted.
-
 Lemma soundness {l} : FMsetEC_SAT (encode_problem l) -> FMsetC_SAT l.
 Proof.
   move=> [ψ]. rewrite -Forall_forall Forall_flat_mapP => Hψ.
@@ -274,230 +153,14 @@ Proof.
   move=> /Hφ Ht /Hφ Hu.
   under eq_lr; by eassumption.
 Qed.
-  
 
-
-
-(*
-(* inject mset_term into poly variables *)
-Fixpoint term_to_nat (t: mset_term) : nat :=
-  match t with
-  | mset_term_zero => nat2_to_nat (0, 0)
-  | mset_term_var x => nat2_to_nat (1, x)
-  | mset_term_plus t u => nat2_to_nat (2, nat2_to_nat ((term_to_nat t), (term_to_nat u)))
-  | mset_term_h t => nat2_to_nat (3, term_to_nat t)
-  end.
-
-Fixpoint nat_to_term
-
-(* decompose mset_term into poly constraints *)
-Fixpoint term_to_polycs (t: mset_term) : list polyc :=
-  match t with
-  | mset_term_zero => [polyc_sum (term_to_nat t) (term_to_nat t) (term_to_nat t)]
-  | mset_term_var x => []
-  | mset_term_plus u v => [polyc_sum (term_to_nat t) (term_to_nat u) (term_to_nat v)]
-  | mset_term_h u => [polyc_prod (term_to_nat t) [0; 1] (term_to_nat u)]
-  end.
-
-Definition mset_eq_to_polycs (t u: mset_term) :=
-  [polyc_sum (term_to_nat t) (term_to_nat mset_term_zero) (term_to_nat u); 
-  (polyc_sum (term_to_nat mset_term_zero) (term_to_nat mset_term_zero) (term_to_nat mset_term_zero))].
-
-(* encode FMsetC_PROBLEM as LPolyNC_PROBLEM *)
-Definition encode_problem (msetcs : FMsetC_PROBLEM) : LPolyNC_PROBLEM :=
-  flat_map (fun '(t, u) => mset_eq_to_polycs t u ++ term_to_polycs t ++ term_to_polycs u) msetcs.
-
-Definition mset_sat (φ : nat -> list nat) (l : FMsetC_PROBLEM) := 
-  Forall (fun '(A, B) => (mset_sem φ A) ≡ (mset_sem φ B)) l.
-
-Lemma mset_satP {φ l} : mset_sat φ l <-> (forall (A B : mset_term), In (A, B) l -> (mset_sem φ A) ≡ (mset_sem φ B)).
+(* many-one reduction from FMsetC to FMsetEC *)
+Theorem FMsetC_to_FMsetEC : FMsetC_SAT ⪯ FMsetEC_SAT.
 Proof.
-  rewrite /mset_sat Forall_forall. constructor.
-  - move=> H A B. apply /H.
-  - move=> H [A B]. apply /H.
+  exists encode_problem.
+  move=> cs. constructor.
+    exact completeness.
+  exact soundness.
 Qed.
 
-Lemma completeness {l} : FMsetC_SAT l -> LPolyNC_SAT (encode_problem l).
-Proof.
-  move=> [φ]. rewrite -mset_satP.
-  rewrite /FMsetC_SAT.
-*)
-
-
-(* list facts *)
-
-Lemma singleton_length {X : Type} {A : list X} : length A = 1 -> exists a, A = [a].
-Proof.
-  case: A.
-    done.
-  move => a A /=. case. move /length_zero_iff_nil => ->. by eexists.
-Qed.
-
-Lemma nil_or_ex_max (A : list nat) : A = [] \/ exists a, In a A /\ Forall (fun b => a >= b) A.
-Proof.
-  elim: A.
-    by left.
-  move=> a A. case.
-    move=> ->. right. exists a. split; by [left | constructor].
-  move=> [b [Hb1 Hb2]]. right.
-  case: (le_lt_dec a b)=> ?.
-  - exists b. split; by [right | constructor].
-  - exists a. split.
-      by left.
-    constructor.
-      done.
-    move: Hb2. apply /Forall_impl => ?. by lia.
-Qed.
-
-(* count_occ facts *)
-Lemma count_occ_app {X : Type} {D : forall x y : X, {x = y} + {x <> y}} {A B c}:
-count_occ D (A ++ B) c = count_occ D A c + count_occ D B c.
-Proof.
-  elim: A B.
-    done.
-  move=> a A IH B /=. rewrite IH. by case: (D a c).
-Qed.
-
-Lemma count_occ_cons {X : Type} {D : forall x y : X, {x = y} + {x <> y}} {A a c}:
-count_occ D (a :: A) c = count_occ D (locked [a]) c + count_occ D A c.
-Proof.
-  rewrite /count_occ /is_left -lock. by case: (D a c).
-Qed.
-
-(* In facts *)
-Lemma in_cons_iff : forall {A : Type} {a b : A} {l : list A}, In b (a :: l) <-> (a = b \/ In b l).
-Proof. by constructor. Qed.
-
-(* Forall facts *)
-Lemma Forall_nil_iff {X: Type} {P: X -> Prop} : Forall P [] <-> True.
-Proof. by constructor. Qed.
-
-Lemma Forall_cons_iff {T: Type} {P: T -> Prop} {a l} :
-  Forall P (a :: l) <-> P a /\ Forall P l.
-Proof.
-  constructor. 
-    move=> H. by inversion H.
-  move=> [? ?]. by constructor.
-Qed.
-
-Lemma Forall_singleton_iff {X: Type} {P: X -> Prop} {x} : Forall P [x] <-> P x.
-Proof.
-  rewrite Forall_cons_iff. by constructor; [case |].
-Qed.
-
-Lemma Forall_app_iff {T: Type} {P: T -> Prop} {A B}: Forall P (A ++ B) <-> Forall P A /\ Forall P B.
-Proof.
-  elim: A.
-    constructor; by [|case].
-  move=> ? ? IH /=. rewrite ? Forall_cons_iff ? IH.
-  by tauto.
-Qed.
-
-(* usage: rewrite ? Forall_norm *)
-Definition Forall_norm := (@Forall_app_iff, @Forall_singleton_iff, @Forall_cons_iff, @Forall_nil_iff).
-
-(* Forall2 facts *)
-Lemma Forall2_nil_rE {X Y: Type} {P: X -> Y -> Prop} {A}: Forall2 P A [] -> A = [].
-Proof. move=> H. by inversion H. Qed.
-
-Lemma Forall2_nil_lE {X Y: Type} {P: X -> Y -> Prop} {A}: Forall2 P [] A -> A = [].
-Proof. move=> H. by inversion H. Qed.
-
-Lemma Forall2_lastP {X Y: Type} {P: X -> Y -> Prop} {A B a b}:
-  Forall2 P (A ++ [a]) (B ++ [b]) <-> Forall2 P A B /\ P a b.
-Proof. 
-  elim: A B => /=.
-    move=> B. constructor.
-      elim: B => /=.
-        move=> H. by inversion H.
-      move=> c B IH H. inversion H. subst.
-      have := Forall2_nil_lE ltac:(eassumption). by move /app_eq_nil => [_].
-    move=> [/Forall2_nil_lE ->] ? /=. by constructor.
-  move=> c A IH. elim=> /=.
-    constructor.
-      move=> H. inversion H. subst.
-      have := Forall2_nil_rE ltac:(eassumption). by move /app_eq_nil => [_].
-    by move=> [/Forall2_nil_rE].
-  move=> d B IH2. constructor.
-    move=> H. inversion H. subst. constructor.
-      constructor.
-        done.
-      have := iffLR (IH B) ltac:(eassumption). by case.
-    have := iffLR (IH B) ltac:(eassumption). by case.
-  move=> [H ?]. inversion H. subst. constructor.
-    done.
-  apply /IH. by constructor.
-Qed.
-
-(* seq facts *)
-Lemma seq_last start length : seq start (S length) = (seq start length) ++ [start + length].
-Proof.
-  have -> : S length = length + 1 by lia.
-  by rewrite seq_app.
-Qed.
-
-(* repeat facts *)
-Lemma repeat_add {X : Type} {x : X} {m n} : repeat x (m + n) = repeat x m ++ repeat x n.
-Proof.
-  elim: m.
-    done.
-  move=> m IH. cbn. by f_equal.
-Qed.
-
-Lemma Forall_repeat {X: Type} {a} {A: list X} : Forall (fun b => a = b) A -> A = repeat a (length A).
-Proof.
-  elim: A.
-    done.
-  move=> b A IH. rewrite Forall_norm => [[? /IH ->]]. subst b.
-  cbn. by rewrite repeat_length.
-Qed.
-
-
-
-(* encode a single H10UC constraint as a list of FMsetC constraints *)
-Definition encode_h10uc '(x, y, z) := encode_constraint x y z.
-
-(* many-one reduction from H10UC to FMsetC *)
-Theorem H10UC_to_FMsetC : H10UC_SAT ⪯ FMsetC_SAT.
-Proof.
-  exists (fun h10ucs => flat_map encode_h10uc h10ucs).
-  move=> h10ucs. constructor.
-  - move=> [φ Hφ]. 
-    exists (construct_valuation φ).
-    elim: h10ucs Hφ.
-      done.
-    move=> [[x y] z] h10cs IH.
-    move /Forall_forall. rewrite Forall_cons_iff. move=> [Hxyz /Forall_forall /IH].
-    move=> {}IH A B.
-    rewrite /flat_map -/(flat_map _) in_app_iff. case; first last.
-      by apply /IH.
-    rewrite /encode_h10uc.
-    have := @encode_constraint_sat φ x y z ltac:(done).
-    rewrite /mset_sat Forall_forall. by apply.
-  - move=> [φ]. rewrite - mset_satP /mset_sat. move=> Hφ.
-    pose ψ := (fun x => length (φ (embed (x, 0, 1)))).
-    exists ψ.
-    rewrite - Forall_forall.
-    elim: h10ucs Hφ.
-      done.
-    move=> [[x y] z] h10ucs IH. rewrite /flat_map -/(flat_map _) Forall_app_iff.
-    rewrite /(encode_h10uc _).
-    move=> [/encode_constraint_spec Hxyz /IH ?].
-    by constructor.
-Qed.
-
-Check H10UC_to_FMsetC.
-(* Print Assumptions H10UC_to_FMsetC. *)
-
-From Undecidability Require Import Problems.TM.
-From Undecidability Require Import Reductions.H10C_to_H10UC.
-
-(* undecidability of FMsetC *)
-Theorem FMsetC_undec : Halt ⪯ FMsetC_SAT.
-Proof.
-  apply (reduces_transitive H10UC_undec).
-  apply H10UC_to_FMsetC.
-Qed.
-
-Check FMsetC_undec.
-(* Print Assumptions FMsetC_undec. *)
+(* Print Assumptions FMsetC_to_FMsetEC. *)
